proofs/talos/lean/Project/Correct/Scalar64/Artifacts.lean
@@ -1,5 +1,0 @@
-import Project.Correct.Scalar64.Artifacts.Affine
-import Project.Correct.Scalar64.Artifacts.Choose
-import Project.Correct.Scalar64.Artifacts.Mix
-import Project.Correct.Scalar64.Artifacts.Helper
-import Project.Correct.Scalar64.Artifacts.Gcd
